WIP(elib): struggling with failure-compatible types

packages/zoe/spec/elib.dfy
@@ -1,26 +1,36 @@
-include "outcome.dfy"
 include "passable.dfy"
 
 module ELib {
-  import opened Outcome
   import opened Passable
 
-  type Value = Passable<Callable, Ref, object>
+  trait Result {
+    predicate IsFailure()
+    function PropagateFailure(): Result
+      requires IsFailure()
+    function Extract(): Value
+      requires !IsFailure()
+  }
+  trait Error extends Result {
+    const message: string
+  }
+  class Fail extends Error {
+    constructor(msg: string) ensures message == msg { message := msg; }
+    predicate IsFailure() { true }
+    function PropagateFailure(): Result { this }
+    function Extract(): Value { Undefined }
+  }
+  type Value = Passable<Callable, Ref, Error>
 
   trait Cap {
-    ghost function Valid(): bool reads this
+    /** "only connectivity begets connectivity" */
+    ghost function CapOK(): bool reads this
     ghost var reach: set<object>
   }
 
-  trait Callable extends Cap {
-    method callAll(verb: string, args: seq<Value>) returns (ret: Outcome<Value>)
-      requires Valid()
-      ensures Valid()
-  }
-
-  class Error {
-    const message: string
-    constructor (m: string) ensures message == m { message := m; }
+  trait {:termination false} Callable extends Cap {
+    method callAll(verb: string, args: seq<Value>) returns (ret: Result)
+      requires CapOK()
+      ensures CapOK()
   }
 
   trait Resolver {
@@ -57,7 +67,7 @@ module ELib {
     }
   }
 
-  trait Ref extends Callable {
+  trait Ref extends Callable, Result {
     static method promise() returns (ref: Ref, resolver: Resolver)
     {
       var buf := new FlexList();
@@ -65,28 +75,52 @@ module ELib {
       resolver := new LocalResolver(ref, buf);
     }
 
-    method sendAll(verb: string, args: seq<Value>) returns (ret: Ref) requires Valid() modifies reach
+    method sendAll(verb: string, args: seq<Value>) returns (ret: Ref) requires CapOK() modifies reach
+    method MoveNext() returns (out: Result)
+  }
+
+  class UnconnectedRef extends Ref {
+    const reason: Error
+    constructor(reason: Error) ensures CapOK() { this.reason := reason; reach := {this, reason}; }
+    ghost function CapOK(): bool reads this { true }
+    predicate IsFailure() { true }
+    function PropagateFailure(): Result { reason }
+    function Extract(): Value { Undefined }
+    method callAll(verb: string, args: seq<Value>) returns (out: Result) {
+      return new Fail("not synchronously callable:" + verb);
+    }
+
+    method sendAll(verb: string, args: seq<Value>) returns (out: Ref) {
+      // doBreakage
+      return this;
+    }
+    method MoveNext() returns (out: Result) {
+      return new Fail("TODO");
+    }
   }
 
   class BufferingRef extends Ref {
+    predicate IsFailure() { false }
+    function PropagateFailure(): Result { this } // impossible
+    function Extract(): Value { String("TODO") } // EVENTUAL. function of state?
+
     var msgs: Opt<FlexList<Message>> // when is this set to None?
-    ghost function Valid(): bool reads this { msgs == None || msgs.value in reach }
+    ghost function CapOK(): bool reads this { msgs == None || msgs.value in reach }
     constructor(buffer: FlexList<Message>)
-      ensures Valid()
+      ensures CapOK()
     {
       this.msgs := Some(buffer);
       reach := { this, buffer };
     }
 
-    method callAll(verb: string, args: seq<Value>) returns (out: Outcome<Value>) {
-      var err := new Error("not synchronously callable:" + verb);
-      return Failure(err);
+    method callAll(verb: string, args: seq<Value>) returns (out: Result) {
+      return new Fail("not synchronously callable:" + verb);
     }
 
     method sendAll(verb: string, args: seq<Value>) returns (result: Ref)
-      requires Valid()
+      requires CapOK()
       modifies reach
-      ensures Valid()
+      ensures CapOK()
     {
       match msgs {
         case Some(m) => {
@@ -99,6 +133,10 @@ module ELib {
         }
       }
     }
+
+    method MoveNext() returns (out: Result) {
+      return new Fail("TODO");
+    }
   }
 
   datatype Opt<T> = None | Some(value: T)
@@ -110,37 +148,43 @@ module ELib {
   datatype Delivery = Pending(vat: Vat, rec: object, res: Resolver, verb: string, args: seq<Value>)
 
   trait Runner {
-    method enqueue(d: Delivery) returns (ret: Outcome<()>)
+    method enqueue(d: Delivery) // TODO: can fail?
+    {
+      print "TODO\n";
+    }
   }
 
-  trait Vat extends Runner {
-    method qSendAll(rec: object, verb: string, args: seq<Value>, resolver: Resolver) returns (ret: Outcome<()>) {
+  trait {:termination false} Vat extends Runner {
+    method qSendAll(rec: object, verb: string, args: seq<Value>, resolver: Resolver) // can fail?
+    {
       var pe := Pending(this, rec, resolver, verb, args);
-      ret := Success(());
+      enqueue(pe);
     }
     method sendAll3(rec: object, verb: string, args: seq<Value>) returns (ret: Ref) {
       var promise, resolver := Ref.promise();
-      var err := qSendAll(rec, verb, args, resolver); // TODO: check error?
+      qSendAll(rec, verb, args, resolver); // TODO: check error?
       ret := promise;
     }
   }
 
-  trait E extends Vat {
+  trait {:termination false} E extends Vat {
+    const theBroken: Ref
+    function broken(): Ref { theBroken }
+
     /**
     ref https://github.com/kpreid/e-on-java/blob/master/src/jsrc/org/erights/e/elib/prim/E.java
      */
-    method callAll(rec: object, verb: string, args: seq<Value>) returns (ret: Outcome<Value>)
-      requires !(rec is Callable) || (rec as Callable).Valid()
+    method callAll(rec: object, verb: string, args: seq<Value>) returns (ret: Result)
+      requires !(rec is Callable) || (rec as Callable).CapOK()
     {
       if (!(rec is Callable)) {
-        var err := new Error("not a function");
-        return Failure(err);
+        return new Fail("not Callable");
       }
       ret := (rec as Callable).callAll(verb, args);
     }
 
     method sendAll(rec: object, verb: string, args: seq<Value>) returns (ret: Ref)
-      requires !(rec is Ref) || (rec as Ref).Valid()
+      requires !(rec is Ref) || (rec as Ref).CapOK()
       modifies if (rec is Ref) then (rec as Ref).reach else {}
     {
       if (rec is Ref) {
